proof done, some cleanup needed

Montanari_Contrasim_Set_Game.thy
@@ -295,7 +295,7 @@ proof (safe)
   qed
 qed
 
-lemma strategy_from_set_contrasim_sound : 
+lemma strategy_from_delay_set_contrasim_sound : 
   assumes
     \<open>contrasim C\<close>
     \<open>C p0 q0\<close>
@@ -385,6 +385,9 @@ proof -
   thus ?thesis using \<open>p = p1\<close> n0_def by auto
 qed
 
+definition delay_x :: "'a list \<Rightarrow> 's \<Rightarrow> 's \<Rightarrow> 's \<Rightarrow> bool" where
+\<open>delay_x A p p0 p1 = (\<exists>p00. p \<Rightarrow>$(butlast A) p00 \<and> p00 =\<rhd>(last A) p0 \<and> p0 \<Rightarrow>^\<tau> p1)\<close>
+
 
 lemma defSimNode_with_prefix_in_play: 
   assumes 
@@ -395,8 +398,8 @@ lemma defSimNode_with_prefix_in_play:
     \<open>sound_strategy f\<close>
     \<open>play \<in> plays_for_strategy f\<close>
     \<open>hd play = AttackerNode p {q}\<close>
-  shows \<open>\<exists>play. ((DefenderSimNode (last A) p1 (dsuccs_seq_rec (rev (butlast A)) {q}))#play) 
-      \<in> plays_for_strategy f\<close> 
+  shows \<open>\<exists>play p0. ((DefenderSimNode (last A) p0 (dsuccs_seq_rec (rev (butlast A)) {q}))#play) 
+      \<in> plays_for_strategy f \<and> delay_x A p p0 p1\<close> 
 proof - 
   have  \<open>\<not>player1_wins play\<close> using assms(4, 6) player0_winning_strategy_def by auto
   hence \<open>(c_set_game_defender_node (hd play) \<and> (\<nexists>p'. c_set_game_moves (hd play) p')) \<Longrightarrow> False\<close> 
@@ -404,7 +407,7 @@ proof -
   hence Def_not_stuck: \<open>c_set_game_defender_node (hd play) \<Longrightarrow> (\<exists>p'. c_set_game_moves (hd play) p')\<close> 
     by auto
   show ?thesis using assms(1-3)
-  proof (induct arbitrary: p1 rule: rev_nonempty_induct[OF assms(1)])
+  proof (induct arbitrary:  p1 rule: rev_nonempty_induct[OF assms(1)])
     case single: (1 a)
     hence \<open>\<not>tau a\<close> using \<open>\<forall>a\<in>set A. a \<noteq> \<tau>\<close> by (simp add: tau_def) 
     hence \<open>p \<Rightarrow>$[a] p1\<close> using single by auto
@@ -412,10 +415,14 @@ proof -
     then obtain p0 where \<open>p =\<rhd>a p0\<close> \<open>p0 \<Rightarrow>^\<tau> p1\<close> using Cons \<open>\<not>tau a\<close> steps.refl by auto
     hence \<open>\<exists>n0. n0  = DefenderSimNode a p0 {q} \<and> c_set_game_moves (AttackerNode p {q}) n0\<close> 
       using assms(4) \<open>\<not> tau a\<close> by simp
-    hence \<open>((DefenderSimNode a p0 {q})#play) \<in> plays_for_strategy f\<close> using assms(6,7)
+    hence  \<open>((DefenderSimNode a p0 {q})#play) \<in> plays_for_strategy f\<close> using assms(6,7)
       by (metis c_set_game_defender_node.simps(1) list.collapse no_empty_plays 
             player1_position_def plays_for_strategy.p1move strategy_plays_subset)
-    then show ?case  by auto
+    hence inplay: \<open>((DefenderSimNode (last [a]) p0  (dsuccs_seq_rec (rev (butlast [a])) {q}))#play) \<in> plays_for_strategy f\<close>
+      by auto
+    have \<open>p  \<Rightarrow>$(butlast [a]) p\<close> by (simp add: steps.refl) 
+    hence \<open>delay_x [a] p p0 p1\<close> using delay_x_def \<open>p =\<rhd>a p0\<close> \<open>p0 \<Rightarrow>^\<tau> p1\<close> by auto
+    then show ?case using inplay by auto
   next
     case snoc: (2 a as)
     hence \<open>\<not>tau a\<close> using \<open>\<forall>a\<in>set A. a \<noteq> \<tau>\<close> by (simp add: tau_def) 
@@ -424,37 +431,43 @@ proof -
     hence \<open>\<exists>p'. p \<Rightarrow>$ as  p' \<and> p' \<Rightarrow>^a  p1\<close> by blast
     hence \<open>\<exists>p'. p \<Rightarrow>$ as  p' \<and> p' \<Rightarrow>a  p1\<close> using  \<open>\<not>tau a\<close> by simp
     then obtain p' where p'_def: \<open>p \<Rightarrow>$ as  p'\<close> and p'_step: \<open>p' \<Rightarrow>a  p1\<close> by auto
-    then obtain play 
-      where play_def: \<open>DefenderSimNode (last as) p' (dsuccs_seq_rec (rev (butlast as)) {q}) # play 
-                \<in> plays_for_strategy f\<close> using snoc by auto
-    hence \<open>DefenderSimNode a2 p' (dsuccs_seq_rec (rev as2) {q}) # play 
+    then obtain p11 where  \<open>p' =\<rhd>a  p11\<close> \<open>p11 \<Rightarrow>^\<tau> p1\<close> using steps.refl \<open>\<not> tau a\<close> tau_tau by blast
+    hence \<open>\<exists>play p0.
+       DefenderSimNode (last as) p0 (dsuccs_seq_rec (rev (butlast as)) {q}) # play
+       \<in> plays_for_strategy f \<and> delay_x as p p0 p'\<close>  using p'_def snoc by auto
+    then obtain play p0
+      where play_def: \<open>DefenderSimNode (last as) p0 (dsuccs_seq_rec (rev (butlast as)) {q}) # play
+       \<in> plays_for_strategy f\<close> \<open>delay_x as p p0 p'\<close> by auto
+
+    hence \<open>DefenderSimNode a2 p0 (dsuccs_seq_rec (rev as2) {q}) # play 
                 \<in> plays_for_strategy f\<close> using as_def by auto
-    then obtain n0 where n0_def: \<open>n0 = DefenderSimNode a2 p' (dsuccs_seq_rec (rev as2) {q})\<close> 
+    then obtain n0 where n0_def: \<open>n0 = DefenderSimNode a2 p0 (dsuccs_seq_rec (rev as2) {q})\<close> 
           and n0_in_play: \<open>n0#play \<in> plays_for_strategy f\<close> by auto
-    hence \<open>\<exists>n1. c_set_game_moves (DefenderSimNode a2 p' (dsuccs_seq_rec (rev as2) {q})) n1\<close> 
+    hence \<open>\<exists>n1. c_set_game_moves (DefenderSimNode a2 p0 (dsuccs_seq_rec (rev as2) {q})) n1\<close> 
       using Def_not_stuck by (meson assms(5) c_set_game_defender_node.simps(2) sound_strategy_def) 
     then obtain n1 
-      where n1_def: \<open>c_set_game_moves (DefenderSimNode a2 p' (dsuccs_seq_rec (rev as2) {q})) n1\<close> 
+      where n1_def: \<open>c_set_game_moves (DefenderSimNode a2 p0 (dsuccs_seq_rec (rev as2) {q})) n1\<close> 
       by auto
-    hence n1_atk: \<open>n1 = AttackerNode p' (succs a2 ((dsuccs_seq_rec (rev as2) {q})))\<close> 
+    hence n1_atk: \<open>n1 = AttackerNode p0 (dsuccs a2 ((dsuccs_seq_rec (rev as2) {q})))\<close> 
       using move_DefSim_to_AtkNode[OF n1_def] by auto
     have n1_in_play: \<open>n1#n0#play \<in> plays_for_strategy f\<close> using n1_def n0_in_play n0_def
       by (metis assms(5) move_DefSim_to_AtkNode c_set_game_defender_node.simps(2) 
           plays_for_strategy.simps sound_strategy_def) 
     then obtain n0' 
-      where n0'_def : \<open>n0' = DefenderSimNode a p1 (succs a2 ((dsuccs_seq_rec (rev as2) {q})))\<close> 
-      and n0'_mov: \<open>c_set_game_moves n1 n0'\<close> using p'_step n1_atk by (simp add: \<open>\<not> tau a\<close>)
+      where n0'_def : \<open>n0' = DefenderSimNode a p11 (dsuccs a2 ((dsuccs_seq_rec (rev as2) {q})))\<close> 
+      and n0'_mov: \<open>c_set_game_moves n1 n0'\<close> using p'_step n1_atk
+      by (metis (no_types, lifting) \<open>\<not> tau a\<close> \<open>p' =\<rhd> a p11\<close> delay_x_def simulation_challenge play_def(2) steps_concat tau_tau)
     hence in_play: \<open>n0'#n1#n0#play \<in> plays_for_strategy f\<close> using n1_in_play
       by (simp add: n1_atk player1_position_def plays_for_strategy.p1move) 
-    hence simnode: \<open>n0' = DefenderSimNode a p1 (succs a2 ((succs_seq_rec(rev as2) {q})))\<close> 
-      using n0'_def n0'_mov by auto
-    hence \<open>n0' = DefenderSimNode a p1 (dsuccs_seq_rec (rev (as2@[a2])) {q})\<close> using simnode by auto
-    hence \<open>n0' = DefenderSimNode a p1 (dsuccs_seq_rec (rev (as)) {q})\<close> using as_def by auto
-    then show ?case using in_play by auto
+    hence \<open>n0' = DefenderSimNode a p11 (dsuccs_seq_rec (rev (as2@[a2])) {q})\<close> using n0'_def  by auto
+    hence n0'_is_defSimNode: \<open>n0' = DefenderSimNode a p11 (dsuccs_seq_rec (rev (as)) {q})\<close> using as_def by auto
+    from \<open>p \<Rightarrow>$ as  p'\<close> \<open>p' =\<rhd>a  p11\<close> \<open>p11 \<Rightarrow>^\<tau> p1\<close> have \<open>delay_x (as@[a]) p p11 p1\<close> 
+      using delay_x_def by auto
+    then show ?case using n0'_is_defSimNode in_play by auto
   qed
 qed
 
-lemma set_contrasim_game_sound: 
+lemma delay_set_contrasim_game_sound: 
   assumes
     \<open>player0_winning_strategy f\<close>
     \<open>sound_strategy f\<close>
@@ -493,51 +506,51 @@ proof (safe)
       by (meson c_set_game_defender_node.simps(3) plays_for_strategy.p0move) 
     then obtain n1' where n1'_mov: \<open>c_set_game_moves n0 n1'\<close> 
       and in_play: \<open>n1'#n0#play \<in> plays_for_strategy f\<close> by auto
-    hence \<open>\<exists>q1. n1' = AttackerNode q1 {p1} \<and> (q1 \<in> succs \<tau> {q})\<close>
+    hence \<open>\<exists>q1. n1' = AttackerNode q1 {p1} \<and> (q1 \<in> hsuccs \<tau> {q})\<close>
       by (metis c_set_game_defender_node.elims(2, 3) c_set_game_moves_no_step(3, 4) swap_answer n0_def) 
     then obtain q1 where q1_def: \<open>n1' = AttackerNode q1 {p1}\<close> 
-      and q_succ: \<open>q1 \<in> succs \<tau> {q}\<close> by auto
-    hence q_tau: \<open>q \<Rightarrow>^\<tau> q1\<close> using succs_def by auto
+      and q_succ: \<open>q1 \<in> hsuccs \<tau> {q}\<close> by auto
+    hence q_tau: \<open>q \<Rightarrow>^\<tau> q1\<close> using hsuccs_def by auto
     from in_play q1_def n0_def have \<open>C q1 p1\<close> unfolding C_def by force 
     then show ?thesis using q_tau Nil by auto 
   next
     case (snoc as a)
     hence \<open>A \<noteq> []\<close> by auto
     hence \<open>\<not>tau a\<close> using \<open>\<forall>a\<in>set A. a \<noteq> \<tau>\<close> snoc  by (simp add: tau_def) 
-    have gotoA: \<open>\<exists>play. ((DefenderSimNode (last A) p1 (dsuccs_seq_rec (rev (butlast A)) {q}))#play) 
-      \<in> plays_for_strategy f\<close> 
-      using defSimNode_with_prefix_in_play \<open>p \<Rightarrow>$A p1\<close> 
-        \<open>\<forall>a\<in>set A. a \<noteq> \<tau>\<close> \<open>A \<noteq> []\<close> assms(1,2) play_def play_hd by auto
+    then obtain A_play p0 where 
+     gotoA: \<open>DefenderSimNode (last A) p0 (dsuccs_seq_rec (rev (butlast A)) {q}) # A_play
+        \<in> plays_for_strategy f\<close> \<open>delay_x A p p0 p1\<close> 
+        using defSimNode_with_prefix_in_play \<open>p \<Rightarrow>$A p1\<close> 
+        \<open>\<forall>a\<in>set A. a \<noteq> \<tau>\<close> \<open>A \<noteq> []\<close> assms(1,2) play_def play_hd by meson
     then obtain Q where Q_def: \<open>Q = dsuccs_seq_rec (rev (butlast A)) {q}\<close> by auto
     hence Q_all: \<open>\<forall>q' \<in> Q.  q \<Rightarrow>$(butlast A) q'\<close> using in_s_implies_word_reachable by auto
-    then obtain n0 where n0_def: \<open>n0 = DefenderSimNode a p1 (dsuccs_seq_rec (rev as) {q})\<close> by auto
-    then obtain A_play 
-      where A_play_def: \<open>n0#A_play \<in> plays_for_strategy f\<close> 
-      using gotoA snoc by auto
+    then obtain n0 where n0_def: \<open>n0 = DefenderSimNode a p0 (dsuccs_seq_rec (rev as) {q}) \<close> by auto
+    hence A_play_def: \<open>n0#A_play \<in> plays_for_strategy f\<close> using gotoA snoc by auto
     then obtain n1 where n1_move: \<open>c_set_game_moves n0 n1\<close>
       using n0_def by (meson assms(2) c_set_game_defender_node.simps(2) sound_strategy_def)
-    hence \<open>n1 = AttackerNode p1 (succs a (dsuccs_seq_rec (rev as) {q}))\<close> 
+    hence \<open>n1 = AttackerNode p0 (dsuccs a (dsuccs_seq_rec (rev as) {q}))\<close> 
       using move_DefSim_to_AtkNode n0_def by blast
-    hence \<open>n1 = AttackerNode p1 (dsuccs_seq_rec (a#(rev as)) {q})\<close>  
-      using succs_seq_rec.simps(2) by auto
-    hence \<open>n1 = AttackerNode p1 (dsuccs_seq_rec (rev (as@[a])) {q})\<close> by auto
-    hence n1_def: \<open>n1 = AttackerNode p1 (dsuccs_seq_rec (rev A) {q})\<close> using snoc by auto
+    hence \<open>n1 = AttackerNode p0 (dsuccs_seq_rec (a#(rev as)) {q})\<close>  
+      using dsuccs_seq_rec.simps(2) by auto
+    hence \<open>n1 = AttackerNode p0 (dsuccs_seq_rec (rev (as@[a])) {q})\<close> by auto
+    hence n1_def: \<open>n1 = AttackerNode p0 (dsuccs_seq_rec (rev A) {q})\<close> using snoc by auto
     hence n1_in_play: \<open>n1#n0#A_play \<in> plays_for_strategy f\<close>
       using n0_def A_play_def n1_move assms(2) move_DefSim_to_AtkNode 
         plays_for_strategy.p0move sound_strategy_def 
       by fastforce 
-    from n1_def obtain n0' where n0'_move: \<open>c_set_game_moves n1 n0'\<close> 
+    from \<open>delay_x A p p0 p1\<close> have \<open>p0 \<Rightarrow>^\<tau> p1\<close> using delay_x_def by auto
+    then obtain n0' where n0'_move: \<open>c_set_game_moves n1 n0'\<close>
       and n0'_def: \<open>n0' = DefenderSwapNode p1 (dsuccs_seq_rec (rev A) {q})\<close>
-      using steps.refl local.swap_challenge tau_tau by blast
+      using  swap_challenge tau_tau n1_def by blast
     hence n0'_in_play: \<open>n0'#n1#n0#A_play \<in> plays_for_strategy f\<close>
       using n1_in_play by (simp add: n1_def player1_position_def plays_for_strategy.p1move) 
     then obtain n1' where n1'_move: \<open>c_set_game_moves n0' n1'\<close>
       and in_strat: \<open>n1' = f(n0'#n1#n0#A_play)\<close> 
       using Def_not_stuck n0'_def  assms(2) sound_strategy_def by auto
-    then obtain q1 where q1_def: \<open>q1 \<in> succs \<tau> (dsuccs_seq_rec (rev A) {q})\<close> 
+    then obtain q1 where q1_def: \<open>q1 \<in> hsuccs \<tau> (dsuccs_seq_rec (rev A) {q})\<close> 
       and n1'_def: \<open>n1'  = AttackerNode q1 {p1}\<close> using n0'_def
       by (metis c_set_game_defender_node.cases c_set_game_moves_no_step(3, 7) swap_answer) 
-    hence \<open>q1 \<in> {q1. \<exists>q0 \<in> (dsuccs_seq_rec (rev A) {q}). q0 \<Rightarrow>^\<tau> q1}\<close> using succs_def by auto
+    hence \<open>q1 \<in> {q1. \<exists>q0 \<in> (dsuccs_seq_rec (rev A) {q}). q0 \<Rightarrow>^\<tau> q1}\<close> using hsuccs_def by auto
     also have \<open>... = {q1. \<exists>q0 \<in> (dsuccs_seq_rec (rev A) {q}). q \<Rightarrow>$A q0 \<and> q0 \<Rightarrow>^\<tau> q1}\<close>
       using in_s_implies_word_reachable by auto
     also have \<open>... \<subseteq> {q1. \<exists>q0 \<in> (dsuccs_seq_rec (rev A) {q}). q \<Rightarrow>$A q1}\<close> 
@@ -566,7 +579,7 @@ proof
       (\<lambda>p q. \<exists>play\<in>plays_for_strategy f.
                  hd play = AttackerNode p {q} \<and>
                  (hd play = initial \<or> (\<exists>P. hd (tl play) = DefenderSwapNode q P)))\<close>
-    using set_contrasim_game_sound by blast
+    using delay_set_contrasim_game_sound by blast
   moreover have \<open>(\<lambda>p q. \<exists>play\<in>plays_for_strategy f.
                  hd play = AttackerNode p {q} \<and>
                  (hd play = initial \<or> (\<exists>P. hd (tl play) = DefenderSwapNode q P))) p q\<close>
@@ -577,7 +590,7 @@ next
     \<open>\<exists> C. contrasim C \<and> C p q\<close>
   thus \<open>(\<exists>f. player0_winning_strategy f \<and> sound_strategy f)\<close>
     using set_contrasim_game_complete[OF _ _ assms]
-         strategy_from_set_contrasim_sound[OF _ _ assms] by blast
+         strategy_from_delay_set_contrasim_sound[OF _ _ assms] by blast
 qed
 
 end
